[SoE] Prove properties of 'find_next_prime'
In particular, the function returns a non-negative value less than
or equal to to size of the sieve, and the corresponding entry
(if it exists) is unmarked. Also, every entry between the current prime
and the "next" prime (or the end of the sieve) *is* marked.

FormalVerifyMisc/CodeChef/Template/Primes.lean
@@ -238,22 +238,46 @@ lemma int32_toInt_add_of_pos_of_dvd_of_lt (m n : Int32)
     rw [← two_mul, Int.pow_succ, mul_comm]
     exact (Int.mul_lt_mul_right (two_pos)).mpr hnlt
 
+-- Useful alternate upper bound on 'n'
+lemma sieve_idx_lt_divs_size
+  {L : ℕ} (S : Sieve L) (n : Int32)
+  (hnnn : 0 ≤ n) (hnlt : n.toInt < (L : ℤ)) :
+  n.toInt.natAbs < S.divs.size := by
+  apply Int.lt_of_ofNat_lt_ofNat
+  rw [S.hsize]
+  convert hnlt
+  have hnnn' := Int32.le_iff_toInt_le.mp hnnn
+  exact Int.ofNat_natAbs_of_nonneg hnnn'
+
+-- General strategy for proving termination when iterating over the sieve
+lemma sieve_termination {L : ℕ} (S : Sieve L) (n m : Int32)
+  (hnpos : 0 < n) (hmpos : 0 < m)
+  (hnlt : n.toInt.natAbs < S.divs.size) (hmle : m ≤ n) :
+  S.divs.size - (n + m).toInt.natAbs < S.divs.size - n.toInt.natAbs := by
+  have hnpos' : 0 < n.toInt := int32_toInt_pos_of_pos hnpos
+  have hmpos' : 0 < m.toInt := int32_toInt_pos_of_pos hmpos
+  have hnub : n.toInt < 2 ^ 30 := int32_toInt_lt_of_lt_divs_size S n hnlt
+  have hmub : m.toInt < 2 ^ 30 :=
+    lt_of_le_of_lt (Int32.le_iff_toInt_le.mp hmle) hnub
+  have hnm : (n + m).toInt = n.toInt + m.toInt := by
+    rw [int32_toInt_add_of_bounds]
+    constructor
+    · exact le_trans (by simp) (le_of_lt (Int.add_lt_add hnpos' hmpos'))
+    · exact Int.add_lt_add hnub hmub
+  rw [hnm]
+  apply Nat.sub_lt_sub_left hnlt
+  apply Int.natAbs_lt_natAbs_of_nonneg_of_lt (le_of_lt hnpos')
+  exact Int.lt_add_of_pos_right _ hmpos'
+
 -- Prove the termination requirements for 'mark_multiple'
 lemma mark_multiple_termination {L : ℕ} (S : Sieve L) (n : Int32)
   (hnpos : 0 < n)
   (hdvd : S.p.toInt ∣ n.toInt)
   (hnlt : n.toInt.natAbs < S.divs.size) :
   S.divs.size - (n + S.p).toInt.natAbs < S.divs.size - n.toInt.natAbs := by
-  have hppos' := int32_toInt_pos_of_pos S.hppos
   have hnpos' := int32_toInt_pos_of_pos hnpos
-  have hnp : (n + S.p).toInt = n.toInt + S.p.toInt := by
-    rw [Int.add_comm, Int32.add_comm]
-    apply int32_toInt_add_of_pos_of_dvd_of_lt S.p n S.hppos hnpos hdvd
-    exact int32_toInt_lt_of_lt_divs_size S _ hnlt
-  rw [hnp]
-  apply Nat.sub_lt_sub_left hnlt
-  apply Int.natAbs_lt_natAbs_of_nonneg_of_lt (le_of_lt hnpos')
-  exact Int.lt_add_of_pos_right _ hppos'
+  apply sieve_termination S _ _ hnpos S.hppos hnlt
+  exact Int32.le_iff_toInt_le.mpr (Int.le_of_dvd hnpos' hdvd)
 
 -- Mark one multiple of 'p' in sieve 'S'
 def mark_multiple {L : ℕ} (S : Sieve L) (n : Int32)
@@ -409,78 +433,202 @@ theorem mark_multiples_verify {L : ℕ} (S : Sieve L) :
   have plei := Int.le_of_dvd hipos' pdvdi
   apply mark_multiple_verify <;> assumption
 
+-- Used in 'find_next_prime' below
+lemma int32_toInt_succ_of_lt_sieve_length {L : ℕ} (S : Sieve L)
+  (n : Int32) (hlt : n.toInt < (L : ℤ)) :
+  (n + 1).toInt = n.toInt + 1 := by
+  apply int32_toInt_succ _ (Int32.lt_iff_toInt_lt.mpr _)
+  apply lt_trans hlt (lt_trans (Int.ofNat_lt_ofNat_of_lt S.hLlt) _)
+  unfold Int32.maxValue; simp
+
+-- Used in 'find_next_prime' below
+lemma int32_lt_succ_of_lt_sieve_length {L : ℕ} (S : Sieve L)
+  (n : Int32) (hlt : n.toInt < (L : ℤ)) :
+  n < n + 1 := by
+  apply Int32.lt_iff_toInt_lt.mpr
+  convert Int.lt_succ n.toInt
+  exact int32_toInt_succ_of_lt_sieve_length S n hlt
+
+-- Prove that 'find_next_prime_impl' (defined below) terminates
+-- This will also be used to prove termination for many related proofs
+lemma find_next_prime_impl_termination
+  {L : ℕ} (S : Sieve L) (n : Int32) (hltn : 1 < n) (nlt : n.toInt < (L : ℤ)) :
+  S.divs.size - (n + 1).toInt.natAbs < S.divs.size - n.toInt.natAbs := by
+  have hnpos : 0 < n := Int32.lt_trans (by simp) hltn
+  have nlt' := sieve_idx_lt_divs_size S n (Int32.le_of_lt hnpos) nlt
+  exact sieve_termination S _ _ hnpos (by simp) nlt' (Int32.le_of_lt hltn)
+
 -- Loop over the entries in the sieve to find the next prime
 def find_next_prime_impl {L : ℕ} (S : Sieve L)
-  (n : Int32) (hltn : 1 < n)
-  (hmark : ∀ (i : ℕ), (plti : S.p.toInt < (i : ℤ)) →
-    (iltn : (i : ℤ) < n.toInt) →
-    (iltL : i < L) →
-    S.divs[i]'(by rwa [S.hsize]) ≠ 0) : Int32 :=
+  (n : Int32) (hltn : 1 < n) : Int32 :=
   if nlt : n.toInt < (L : ℤ) then
-  (fun hns : (n + 1).toInt = n.toInt + 1 ↦
-    if h : S.divs[n.toInt.natAbs]'(by
+  if h : S.divs[n.toInt.natAbs]'(by
       apply Int.lt_of_ofNat_lt_ofNat
       convert S.hsize ▸ nlt
       apply Int.natAbs_of_nonneg (le_of_lt _)
       apply lt_trans _ (Int32.lt_iff_toInt_lt.mp hltn); simp
-    ) = 0 then n else
-    find_next_prime_impl S (n + 1) (by
-      apply Int32.lt_iff_toInt_lt.mpr
-      rw [hns]
-      apply Int.lt_add_of_le_of_pos _ (by simp)
-      exact le_of_lt (Int32.lt_iff_toInt_lt.mp hltn)
-    ) (by
-        intro i plti iltn iltL
-        rw [hns] at *
-        by_cases hinabs : i = n.toInt.natAbs
-        · rwa [getElem_congr_idx hinabs]
-        apply hmark i plti _ iltL
-        apply lt_of_le_of_ne (Int.le_of_lt_add_one iltn)
-        contrapose! hinabs
-        apply Int.ofNat_inj.mp
-        rw [hinabs, Int.ofNat_natAbs_of_nonneg]
-        apply le_of_lt
-        apply lt_trans _ (Int32.lt_iff_toInt_lt.mp hltn); simp
-    )
-  ) (by
-    apply int32_toInt_succ
-    apply Int32.lt_iff_toInt_lt.mpr (lt_trans nlt _)
-    apply lt_trans (Int.ofNat_lt_ofNat_of_lt S.hLlt)
-    unfold Int32.maxValue; simp
+  ) = 0 then n else
+  find_next_prime_impl S (n + 1) (by
+    apply Int32.lt_trans hltn
+    exact int32_lt_succ_of_lt_sieve_length S _ nlt
   ) else Int32.ofInt (L : ℤ)
 termination_by S.divs.size - n.toInt.natAbs
 decreasing_by
-  have hnn : 0 ≤ n.toInt := by
-    apply le_of_lt
-    apply lt_trans _ (Int32.lt_iff_toInt_lt.mp hltn); simp
-  rw [hns, Int.natAbs_add_of_nonneg]
-  · rw [← Nat.sub_sub]
-    apply Nat.sub_lt
-    · apply Nat.sub_pos_of_lt
-      apply Int.lt_of_ofNat_lt_ofNat
-      rwa [S.hsize, Int.ofNat_natAbs_of_nonneg]
-      assumption
-    · simp
-  · assumption
-  · simp
+  apply find_next_prime_impl_termination <;> assumption
 
+-- Starting with the current prime, search for the next prime
 def find_next_prime {L : ℕ} (S : Sieve L) : Int32 :=
-  (fun hns : (S.p + 1).toInt = S.p.toInt + 1 ↦
-    find_next_prime_impl S (S.p + 1) (by
-      apply Int32.lt_iff_toInt_lt.mpr
-      rw [hns]; simp
-      exact Int32.lt_iff_toInt_lt.mp S.hppos
-    ) (by
-      intro i plti iltn iltL
-      rw [hns] at iltn
-      exact False.elim (not_lt_of_ge (Int.le_of_lt_add_one iltn) plti)
-    )
-  ) (by
-    apply int32_toInt_succ
+  find_next_prime_impl S (S.p + 1) (by
     apply Int32.lt_iff_toInt_lt.mpr
-    apply lt_trans S.hplt
-    apply lt_trans (Int.ofNat_lt_ofNat_of_lt S.hLlt)
-    unfold Int32.maxValue; simp
+    rw [int32_toInt_succ_of_lt_sieve_length S _ S.hplt]; simp
+    exact Int32.lt_iff_toInt_lt.mp S.hppos
   )
+
+-- 'find_next_prime_impl' always returns a non-negative integer
+theorem find_next_prime_impl_nonneg {L : ℕ} (S : Sieve L)
+  (n : Int32) (hltn : 1 < n) :
+  0 ≤ (find_next_prime_impl S n hltn).toInt := by
+  unfold find_next_prime_impl; dsimp
+  split_ifs with h₀ h₁
+  · exact le_of_lt (lt_trans (by simp) (Int32.lt_iff_toInt_lt.mp hltn))
+  · apply find_next_prime_impl_nonneg
+  · have Lnn := Int.natCast_nonneg L
+    have ltL : -2^31 ≤ (L : ℤ) := le_trans (by simp) Lnn
+    rwa [Int32.toInt_ofInt_of_le ltL]
+    exact lt_trans (Int.ofNat_lt_ofNat_of_lt S.hLlt) (by simp)
+termination_by S.divs.size - n.toInt.natAbs
+decreasing_by
+  apply find_next_prime_impl_termination <;> assumption
+
+-- 'find_next_prime' always returns a non-negative integer
+theorem find_next_prime_nonneg {L : ℕ} (S : Sieve L) :
+  0 ≤ (find_next_prime S).toInt := by
+  unfold find_next_prime
+  apply find_next_prime_impl_nonneg
+
+-- For the length of the sieve, Int32.ofInt and Int32.toInt are inverses
+lemma sieve_length_toInt_ofInt {L : ℕ} (S : Sieve L) :
+  (Int32.ofInt (L : ℤ)).toInt = (L : ℤ) := by
+  apply Int32.toInt_ofInt_of_le
+  · exact le_trans (by simp) (Int.natCast_nonneg L)
+  · exact lt_trans (Int.ofNat_lt_ofNat_of_lt S.hLlt) (by simp)
+
+-- 'find_next_prime_impl' finds an unmarked entry in the sieve
+-- if its search doesn't reach the end of the sieve
+theorem find_next_prime_impl_unmarked {L : ℕ} (S : Sieve L)
+  (n : Int32) (hltn : 1 < n) :
+  (fun p (pnn : 0 ≤ p) ↦ (h : p.toInt < (L : ℤ)) →
+    S.divs[p.toInt.natAbs]'(sieve_idx_lt_divs_size S p pnn h) = 0
+  ) (find_next_prime_impl S n hltn) (by
+    apply Int32.le_iff_toInt_le.mpr
+    exact find_next_prime_impl_nonneg S n hltn
+  ) := by
+  dsimp
+  intro h
+  unfold find_next_prime_impl; dsimp
+  split_ifs with h₀ h₁
+  · exact h₁
+  · unfold find_next_prime_impl at h; dsimp at h
+    rw [dif_pos h₀, if_neg h₁] at h
+    apply find_next_prime_impl_unmarked
+    assumption
+  · unfold find_next_prime_impl at h; dsimp at h
+    rw [dif_neg h₀] at h
+    absurd h; push_neg
+    apply Int.le_of_eq; symm
+    exact sieve_length_toInt_ofInt S
+termination_by S.divs.size - n.toInt.natAbs
+decreasing_by
+  apply find_next_prime_impl_termination <;> assumption
+
+-- 'find_next_prime' finds an unmarked entry in the sieve
+-- if its search doesn't reach the end of the sieve
+theorem find_next_prime_unmarked {L : ℕ} (S : Sieve L) :
+  (fun p (pnn : 0 ≤ p) ↦ (h : p.toInt < (L : ℤ)) →
+    S.divs[p.toInt.natAbs]'(
+      sieve_idx_lt_divs_size S p pnn h
+    ) = 0
+  ) (find_next_prime S) (by
+    apply Int32.le_iff_toInt_le.mpr
+    exact find_next_prime_nonneg S
+  ) := by
+  dsimp
+  intro h
+  unfold find_next_prime at *
+  apply find_next_prime_impl_unmarked
+  assumption
+
+-- The value of 'find_next_prime_impl' does not exceed 'L'
+theorem find_next_prime_impl_ub
+  {L : ℕ} (S : Sieve L) (n : Int32) (hltn : 1 < n) :
+  (find_next_prime_impl S n hltn).toInt ≤ (L : ℤ) := by
+  unfold find_next_prime_impl; dsimp
+  split_ifs with h₀ h₁
+  · exact le_of_lt h₀
+  · apply find_next_prime_impl_ub
+  · apply Int.le_of_eq
+    exact sieve_length_toInt_ofInt S
+termination_by S.divs.size - n.toInt.natAbs
+decreasing_by
+  apply find_next_prime_impl_termination <;> assumption
+
+-- The value of 'find_next_prime' does not exceed 'L'
+theorem find_next_prime_ub {L : ℕ} (S : Sieve L) :
+  (find_next_prime S).toInt ≤ (L : ℤ) := by
+  unfold find_next_prime
+  apply find_next_prime_impl_ub
+
+-- Every entry between the starting point of the search and
+-- the value returned by 'find_next_prime_impl' is marked
+theorem find_next_prime_impl_first_unmarked
+  {L : ℕ} (S : Sieve L) (n : Int32) (hltn : 1 < n) :
+  ∀ (i : ℕ), n.toInt ≤ (i : ℤ) →
+  (ilt : (i : ℤ) < (find_next_prime_impl S n hltn).toInt) →
+  S.divs[i]'(by
+    rw [S.hsize]
+    apply Int.lt_of_ofNat_lt_ofNat (lt_of_lt_of_le ilt _)
+    apply find_next_prime_impl_ub
+  ) ≠ 0 := by
+  intro i nlei ilt
+  have ilt' : i < L := by
+    apply Int.lt_of_ofNat_lt_ofNat
+    apply lt_of_lt_of_le ilt
+    apply find_next_prime_impl_ub
+  unfold find_next_prime_impl at ilt; dsimp at ilt
+  split_ifs at ilt with h₀ h₁
+  · absurd nlei; push_neg
+    assumption
+  · by_cases hni : n.toInt = (i : ℤ)
+    · convert h₁
+      rw [hni]; simp
+    have hnlti : n.toInt < (i : ℤ) := lt_of_le_of_ne nlei hni
+    have hltns : 1 < n + 1 := by
+      apply Int32.lt_trans hltn
+      exact int32_lt_succ_of_lt_sieve_length S n h₀
+    apply find_next_prime_impl_first_unmarked S (n + 1) hltns i _ ilt
+    rw [int32_toInt_succ_of_lt_sieve_length S n h₀]
+    exact Int.add_one_le_of_lt hnlti
+  · absurd nlei; push_neg
+    apply lt_of_lt_of_le _ (le_of_not_gt h₀)
+    exact Int.ofNat_lt_ofNat_of_lt ilt'
+termination_by S.divs.size - n.toInt.natAbs
+decreasing_by
+  apply find_next_prime_impl_termination <;> assumption
+
+-- Every entry between the starting point of the search and
+-- the value returned by 'find_next_prime_impl' is marked
+theorem find_next_prime_first_unmarked
+  {L : ℕ} (S : Sieve L) :
+  ∀ (i : ℕ), S.p.toInt + 1 ≤ (i : ℤ) →
+  (ilt : (i : ℤ) < (find_next_prime S).toInt) →
+  S.divs[i]'(by
+    rw [S.hsize]
+    apply Int.lt_of_ofNat_lt_ofNat (lt_of_lt_of_le ilt _)
+    apply find_next_prime_ub
+  ) ≠ 0 := by
+  intro i plti ilt
+  unfold find_next_prime at ilt
+  rw [← int32_toInt_succ_of_lt_sieve_length S S.p S.hplt] at plti
+  apply find_next_prime_impl_first_unmarked S (S.p + 1) _ i plti ilt
 
 end CodeChef
